uniform presentation of normalizing, normal, and simple HOSemiU

theories/SemiUnification/HOSemiU.v
@@ -29,45 +29,84 @@ Inductive step : term -> term -> Prop :=
   | step_PiL P P' Q: step P P' -> step (Pi P Q) (Pi P' Q)
   | step_PiR P Q Q': step Q Q' -> step (Pi P Q) (Pi P Q').
 
+(* beta-equivalence is the reflexive, symmetric, transitive closure 
+  of the single-step beta reduction *)
+Definition eq_beta := clos_refl_sym_trans term step.
+
+(* a valuation assigns terms to term variables *)
+Definition valuation : Type := nat -> term.
+
+(* inequality: P ≤ Q *)
+Definition inequality : Type := (term * term).
+
+(* terms which satisfy property p *)
+(* for example, "p" can be "normalizing", "normal", or "simple" *)
+Definition term' (p : term -> Prop) := { P : term | p P }.
+
+(* inequality: P ≤ Q where P and Q satisfy property p *)
+Definition inequality' (p : term -> Prop) : Type := (term' p * term' p).
+
+(* a valuation assigns terms with property p to term variables *)
+Definition valuation' (p : term -> Prop) : Type := nat -> term' p.
+
+(* erase term annotation *)
+Definition trim_term' {p : term -> Prop} : term' p -> term := fun P' => proj1_sig P'.
+
+(* erase inequality annotation *)
+Definition trim_inequality' {p : term -> Prop} : inequality' p -> inequality := 
+  fun '(P', Q') => (trim_term' P', trim_term' Q').
+
+(* erase valuation annotations *)
+Definition trim_valuation' {p : term -> Prop} : valuation' p -> valuation := 
+  fun φ' => fun x => trim_term' (φ' x).
+
+(* substitution function "subst_term" is defined in pts.v *)
+
+(* Higher-order Semi-unification Definition *)
+
+(* φ solves P ≤ Q, if there is ψ such that ψ (φ (P)) =β φ (Q) *)
+(* property p is trimmed before substitution *)
+Definition solution {p : term -> Prop} (φ' : valuation' p) : inequality' p -> Prop := 
+  fun '(P', Q') => 
+    exists (ψ' : valuation' p), 
+      let '(P, Q) := (trim_term' P', trim_term' Q') in
+      let φ := trim_valuation' φ' in
+      let ψ := trim_valuation' ψ' in
+      eq_beta (subst_term ψ (subst_term φ P)) (subst_term φ Q).
+
+(* Higher-order Semi-unification *)
+(* is there a valuation φ that solves all inequalities? *)
+(* for example, property "p" can be "normalizing", "normal", or "simple" *)
+Definition HOSemiU (p : term -> Prop) : list (inequality' p) -> Prop := 
+  fun cs => exists (φ : valuation' p), forall (c : inequality' p), In c cs -> solution φ c.
+
 (* a term is (strongly) normalizing if it only allows for finite reduction chains *)
 Definition normalizing (P : term) : Prop := 
   Acc (transp term step) P.
+
+(* Higher-order Semi-unification for strongly normalizing terms *)
+Definition HOSemiU_SN := HOSemiU normalizing.
 
 (* a term is normal if it is not reducible *)
 Definition normal (P : term) : Prop :=
   forall Q, not (step P Q).
 
-(* beta-equivalence is the reflexive, symmetric, transitive closure 
-  of the single-step beta reduction *)
-Definition eq_beta := clos_refl_sym_trans term step.
+(* Higher-order Semi-unification for terms in normal form *)
+Definition HOSemiU_NF := HOSemiU normal.
 
-(* a valuation assigns terms with property p to term variables *)
-Definition valuation (p : term -> Prop) : Type := nat -> { P : term | p P }.
+(* notion of a simple type represented by a term
+  P, Q ::= x | Pi (x : P). Q (where x is not free in Q) *)
+Fixpoint simple (P: term) :=
+  match P with
+  | var _ => True
+  | const _ => False 
+  | app P Q => False
+  | lam P Q => False
+  | Pi P Q => (* Pi (x : P). Q is simple iff *)
+      simple P /\ (* P is simple *)
+      simple Q /\ (* Q is simple *)
+      exists Q', Q = ren_term shift Q' (* x does not occur free in Q *) 
+  end.
 
-(* substitution function "subst_term" is defined in pts.v *)
-
-(* replace free variables by assigned terms with property p *)
-(* for example, p can be "normal_form" or "simple" *)
-Definition substitute {p : term -> Prop} (φ : valuation p) (P : term) : term :=
-  subst_term (fun x => proj1_sig (φ x)) P.
-
-(* Higher-order Semi-unification Definition *)
-
-(* inequality: s ≤ t *)
-Definition inequality : Type := (term * term).
-
-(* φ solves s ≤ t, if there is ψ such that ψ (φ (s)) =β φ (s) *)
-(* property p in the range of φ is the same as in the range of ψ *)
-Definition solution {p : term -> Prop} (φ : valuation p) : inequality -> Prop := 
-  fun '(P, Q) => exists (ψ : valuation p), 
-    eq_beta (substitute ψ (substitute φ P)) (substitute φ Q).
-
-(* Higher-order Semi-unification *)
-(* is there a normalizing valuation φ that solves all inequalities? *)
-Definition HOSemiU (cs: list inequality) := 
-  exists (φ: valuation normalizing), forall (c: inequality), In c cs -> solution φ c.
-
-(* Higher-order Semi-unification *)
-(* is there a normal valuation φ that solves all inequalities? *)
-Definition HOSemiU' (cs: list inequality) := 
-  exists (φ: valuation normal), forall (c: inequality), In c cs -> solution φ c.
+(* Higher-order Semi-unification for simple terms *)
+Definition HOSemiU_SIM := HOSemiU simple.
